Show reading from shared borrows
This (finally) requries us to add thread-local tokens to various judgments

theories/typing/programs.v
@@ -11,7 +11,7 @@ Section typing.
   (* This is an iProp because it is also used by the function type. *)
   Definition typed_body (E : elctx) (L : llctx) (C : cctx) (T : tctx)
                         (e : expr) : iProp Σ :=
-    (∀ tid qE, heap_ctx -∗ lft_ctx -∗ elctx_interp E qE -∗ llctx_interp L 1 -∗
+    (∀ tid qE, heap_ctx -∗ lft_ctx -∗ na_own tid ⊤ -∗ elctx_interp E qE -∗ llctx_interp L 1 -∗
                (elctx_interp E qE -∗ cctx_interp tid C) -∗ tctx_interp tid T -∗
                WP e {{ _, cont_postcondition }})%I.
   Global Arguments typed_body _ _ _ _ _%E.
@@ -32,17 +32,18 @@ Section typing.
     Proper (flip (cctx_incl E) ==> flip (tctx_incl E L) ==> eq ==> (⊢)) (typed_body E L).
   Proof.
     intros C1 C2 HC T1 T2 HT e ? <-. iIntros "H".
-    iIntros (tid qE) "#HEAP #LFT HE HL HC HT".
+    iIntros (tid qE) "#HEAP #LFT Htl HE HL HC HT".
     iMod (HT with "LFT HE HL HT") as "(HE & HL & HT)".
-    iApply ("H" with "HEAP LFT HE HL [HC] HT").
+    iApply ("H" with "HEAP LFT Htl HE HL [HC] HT").
     iIntros "HE". by iApply (HC with "LFT HC").
   Qed.
 
   (** Instruction *)
   Definition typed_instruction (E : elctx) (L : llctx)
              (T1 : tctx) (e : expr) (T2 : val → tctx) : Prop :=
-    ∀ tid qE, heap_ctx -∗ lft_ctx -∗ elctx_interp E qE -∗ llctx_interp L 1 -∗ tctx_interp tid T1 -∗
-                   WP e {{ v, elctx_interp E qE ∗ llctx_interp L 1 ∗ tctx_interp tid (T2 v) }}.
+    ∀ tid qE, heap_ctx -∗ lft_ctx -∗ na_own tid ⊤ -∗
+              elctx_interp E qE -∗ llctx_interp L 1 -∗ tctx_interp tid T1 -∗ 
+                   WP e {{ v, na_own tid ⊤ ∗ elctx_interp E qE ∗ llctx_interp L 1 ∗ tctx_interp tid (T2 v) }}.
   Global Arguments typed_instruction _ _ _ _%E _.
 
   (** Writing and Reading **)
@@ -60,9 +61,9 @@ Section typing.
      fraction was given). So we go with the definition that is easier to prove. *)
   Definition typed_read (E : elctx) (L : llctx) (ty1 ty ty2 : type) : Prop :=
     ∀ v tid F qE qL, lftE ∪ (↑lrustN) ⊆ F →
-      lft_ctx -∗ elctx_interp E qE -∗ llctx_interp L qL -∗ ty1.(ty_own) tid [v] ={F}=∗
+      lft_ctx -∗ na_own tid F -∗ elctx_interp E qE -∗ llctx_interp L qL -∗ ty1.(ty_own) tid [v] ={F}=∗
         ∃ (l : loc) vl q, ⌜v = #l⌝ ∗ l ↦∗{q} vl ∗ ▷ ty.(ty_own) tid vl ∗
-          (l ↦∗{q} vl ={F}=∗ elctx_interp E qE ∗ llctx_interp L qL ∗ ty2.(ty_own) tid [v]).
+          (l ↦∗{q} vl ={F}=∗ na_own tid F ∗ elctx_interp E qE ∗ llctx_interp L qL ∗ ty2.(ty_own) tid [v]).
 End typing.
 
 Notation typed_instruction_ty E L T1 e ty := (typed_instruction E L T1 e (λ v : val, [TCtx_hasty v ty])).
@@ -76,11 +77,11 @@ Section typing_rules.
     (∀ v : val, typed_body E L C (T2 v ++ T) (subst' xb v e')) →
     typed_body E L C (T1 ++ T) (let: xb := e in e').
   Proof.
-    iIntros (Hc He He' tid qE) "#HEAP #LFT HE HL HC HT". rewrite tctx_interp_app.
-    iDestruct "HT" as "[HT1 HT]". wp_bind e. iApply (wp_wand with "[HE HL HT1]").
-    { iApply (He with "HEAP LFT HE HL HT1"). }
-    iIntros (v) "/= (HE & HL & HT2)". iApply wp_let; first wp_done. iModIntro.
-    iApply (He' with "HEAP LFT HE HL HC [HT2 HT]"). rewrite tctx_interp_app. by iFrame.
+    iIntros (Hc He He' tid qE) "#HEAP #LFT Htl HE HL HC HT". rewrite tctx_interp_app.
+    iDestruct "HT" as "[HT1 HT]". wp_bind e. iApply (wp_wand with "[HE HL HT1 Htl]").
+    { iApply (He with "HEAP LFT Htl HE HL HT1"). }
+    iIntros (v) "/= (Htl & HE & HL & HT2)". iApply wp_let; first wp_done. iModIntro.
+    iApply (He' with "HEAP LFT Htl HE HL HC [HT2 HT]"). rewrite tctx_interp_app. by iFrame.
   Qed.
   
   Lemma type_assign E L ty1 ty ty1' p1 p2 :
@@ -88,7 +89,7 @@ Section typing_rules.
     typed_instruction E L [TCtx_hasty p1 ty1; TCtx_hasty p2 ty] (p1 <- p2)
                       (λ _, [TCtx_hasty p1 ty1']).
   Proof.
-    iIntros (Hwrt tid qE) "#HEAP #LFT HE HL".
+    iIntros (Hwrt tid qE) "#HEAP #LFT $ HE HL".
     rewrite tctx_interp_cons tctx_interp_singleton. iIntros "[Hp1 Hp2]".
     wp_bind p1. iApply (wp_hasty with "Hp1"). iIntros (v1) "% Hown1".
     wp_bind p2. iApply (wp_hasty with "Hp2"). iIntros (v2) "_ Hown2".
@@ -108,9 +109,9 @@ Section typing_rules.
     typed_instruction E L [TCtx_hasty p ty1] (!p)
                       (λ v, [TCtx_hasty p ty1'; TCtx_hasty v ty]).
   Proof.
-    iIntros (Hsz Hread tid qE) "#HEAP #LFT HE HL Hp". rewrite tctx_interp_singleton.
+    iIntros (Hsz Hread tid qE) "#HEAP #LFT Htl HE HL Hp". rewrite tctx_interp_singleton.
     wp_bind p. iApply (wp_hasty with "Hp"). iIntros (v) "% Hown".
-    iMod (Hread with "* LFT HE HL Hown") as (l vl q) "(% & Hl & Hown & Hclose)"; first done.
+    iMod (Hread with "* LFT Htl HE HL Hown") as (l vl q) "(% & Hl & Hown & Hclose)"; first done.
     subst v. iAssert (▷⌜length vl = 1%nat⌝)%I with "[#]" as ">%".
     { rewrite -Hsz. iApply ty_size_eq. done. }
     destruct vl as [|v [|]]; try done.
