theories/typing/bool.v
@@ -19,7 +19,7 @@ Section typing.
   Lemma type_bool (b : Datatypes.bool) E L :
     typed_instruction_ty E L [] #b bool.
   Proof.
-    iIntros (tid qE) "_ _ $ $ _". wp_value.
+    iIntros (tid qE) "_ _ $ $ $ _". wp_value.
     rewrite tctx_interp_singleton tctx_hasty_val. iExists _. done.
   Qed.
 
@@ -28,12 +28,12 @@ Section typing.
     typed_body E L C (TCtx_hasty p bool :: T) (if: p then e1 else e2).
   Proof.
     (* FIXME why can't I merge these two iIntros? *)
-    iIntros (He1 He2). iIntros (tid qE) "#HEAP #LFT HE HL HC".
+    iIntros (He1 He2). iIntros (tid qE) "#HEAP #LFT Htl HE HL HC".
     rewrite tctx_interp_cons. iIntros "[Hp HT]".
     wp_bind p. iApply (wp_hasty with "Hp"). iIntros (v) "_ Hown".
     iDestruct "Hown" as (b) "Hv". iDestruct "Hv" as %[=->].
     destruct b; wp_if.
-    - iApply (He1 with "HEAP LFT HE HL HC HT").
-    - iApply (He2 with "HEAP LFT HE HL HC HT").
+    - iApply (He1 with "HEAP LFT Htl HE HL HC HT").
+    - iApply (He2 with "HEAP LFT Htl HE HL HC HT").
   Qed.
 End typing.
