theories/typing/cont.v
@@ -12,10 +12,10 @@ Section typing.
     tctx_incl E L T (T' args) →
     typed_body E L [CCtx_iscont k L n T'] T (k (of_val <$> (args : list _))).
   Proof.
-    iIntros (Hincl tid qE) "#HEAP #LFT HE HL HC HT".
+    iIntros (Hincl tid qE) "#HEAP #LFT Htl HE HL HC HT".
     iMod (Hincl with "LFT HE HL HT") as "(HE & HL & HT)".
     iSpecialize ("HC" with "HE * []"); first by (iPureIntro; apply elem_of_list_singleton).
-    simpl. iApply ("HC" with "* HL HT").
+    simpl. iApply ("HC" with "* Htl HL HT").
   Qed.
 
   Lemma type_cont {n} E L1 L2 C T T' kb (argsb : vec binder n) e1 econt e2 :
@@ -25,16 +25,16 @@ Section typing.
     (∀ k, typed_body E (L1 ++ L2) (CCtx_iscont k L1 n T' :: C) T (subst' kb k e2)) →
     typed_body E (L1 ++ L2) C T (let: kb := e1 in e2).
   Proof.
-    iIntros (-> Hc1 Hc2 Hecont He2 tid qE) "#HEAP #LFT HE HL HC HT". iApply wp_let'.
+    iIntros (-> Hc1 Hc2 Hecont He2 tid qE) "#HEAP #LFT Htl HE HL HC HT". iApply wp_let'.
     { simpl. rewrite decide_left. done. }
-    iModIntro. iApply (He2 with "* HEAP LFT HE HL [HC] HT"). clear He2.
+    iModIntro. iApply (He2 with "* HEAP LFT Htl HE HL [HC] HT"). clear He2.
     iIntros "HE". iLöb as "IH". iIntros (x) "H".
     iDestruct "H" as %[->|?]%elem_of_cons; last by iApply ("HC" with "HE *").
-    iIntros (args) "HL HT". iApply wp_rec; try done.
+    iIntros (args) "Htl HL HT". iApply wp_rec; try done.
     { apply Forall_of_val_is_val. }
     { rewrite -vec_to_list_map -subst_vec_eq. eauto. }
     (* FIXME: iNext here unfolds things in the context. *)
-    iNext. iApply (Hecont with "* HEAP LFT HE HL [HC] HT").
+    iNext. iApply (Hecont with "* HEAP LFT Htl HE HL [HC] HT").
     by iApply "IH".
   Qed.
 
