theories/typing/product.v
@@ -13,11 +13,11 @@ Section product.
 
   Global Instance unit_copy : Copy unit.
   Proof.
-    split. by apply _. iIntros (????????) "_ _ $ Htok".
+    split. by apply _. iIntros (????????) "_ _ Htok $".
     iDestruct (na_own_acc with "Htok") as "[$ Htok]"; first set_solver+.
     iExists 1%Qp. iModIntro. iSplitR.
     { iExists []. iSplitL; last by auto. rewrite heap_mapsto_vec_nil. auto. }
-    iIntros "_ Htok2". iApply "Htok". done.
+    iIntros "Htok2 _". iApply "Htok". done.
   Qed.
 
   Global Instance unit_send : Send unit.
@@ -89,10 +89,10 @@ Section product.
     Copy (product2 ty1 ty2).
   Proof.
     split; first (intros; apply _).
-    intros κ tid E F l q ? HF. iIntros "#LFT [H1 H2] [Htok1 Htok2] Htl".
-    iMod (@copy_shr_acc with "LFT H1 Htok1 Htl") as (q1) "(H1 & Htl & Hclose1)"; first set_solver.
+    intros κ tid E F l q ? HF. iIntros "#LFT [H1 H2] Htl [Htok1 Htok2]".
+    iMod (@copy_shr_acc with "LFT H1 Htl Htok1") as (q1) "(Htl & H1 & Hclose1)"; first set_solver.
     { rewrite <-HF. apply shr_locsE_subseteq. simpl. clear. omega. }
-    iMod (@copy_shr_acc with "LFT H2 Htok2 Htl") as (q2) "(H2 & Htl & Hclose2)"; first set_solver.
+    iMod (@copy_shr_acc with "LFT H2 Htl Htok2") as (q2) "(Htl & H2 & Hclose2)"; first set_solver.
     { move: HF. rewrite /= -plus_assoc shr_locsE_shift.
       assert (shr_locsE l (ty_size ty1) ⊥ shr_locsE (shift_loc l (ty_size ty1)) (ty_size ty2 + 1))
              by exact: shr_locsE_disj.
@@ -109,7 +109,7 @@ Section product.
     iDestruct "H↦1" as "[H↦1 H↦1f]". iDestruct "H↦2" as "[H↦2 H↦2f]".
     iIntros "!>". iSplitL "H↦1 H1 H↦2 H2".
     - iNext. iSplitL "H↦1 H1". iExists vl1. by iFrame. iExists vl2. by iFrame.
-    - iIntros "[H1 H2] Htl". iDestruct ("Htlclose" with "Htl") as "Htl".
+    - iIntros "Htl [H1 H2]". iDestruct ("Htlclose" with "Htl") as "Htl".
       iDestruct "H1" as (vl1') "[H↦1 H1]". iDestruct "H2" as (vl2') "[H↦2 H2]".
       iAssert (▷ ⌜length vl1' = ty1.(ty_size)⌝)%I with "[#]" as ">%".
       { iNext. by iApply ty_size_eq. }
@@ -118,8 +118,8 @@ Section product.
       iCombine "H↦1" "H↦1f" as "H↦1". iCombine "H↦2" "H↦2f" as "H↦2".
       rewrite !heap_mapsto_vec_op; try by congruence.
       iDestruct "H↦1" as "[_ H↦1]". iDestruct "H↦2" as "[_ H↦2]".
-      iMod ("Hclose2" with "[H2 H↦2] Htl") as "[$ Htl]". by iExists _; iFrame.
-      iMod ("Hclose1" with "[H1 H↦1] Htl") as "[$$]". by iExists _; iFrame. done.
+      iMod ("Hclose2" with "Htl [H2 H↦2]") as "[Htl $]". by iExists _; iFrame.
+      iMod ("Hclose1" with "Htl [H1 H↦1]") as "[$$]". by iExists _; iFrame. done.
   Qed.
 
   Global Instance product2_send `{!Send ty1} `{!Send ty2} :
